src/opt/ReorderBase.v
@@ -25,15 +25,6 @@ Require Import Semantics.
 Set Implicit Arguments.
 
 
-Ltac committac :=
-  repeat
-    (try match goal with
-         | [|- Snapshot.le (Snapshot.join _ _) _] =>
-           apply Snapshot.join_spec
-         | [|- Snapshot.le (Snapshot.incr_reads _ _ _) _] =>
-           apply Snapshot.incr_reads_spec
-         end; ss).  
-
 Lemma reorder_read_read
       loc1 ts1 val1 released1 ord1
       loc2 ts2 val2 released2 ord2
@@ -45,12 +36,11 @@ Lemma reorder_read_read
       (WF0: Local.wf th0 mem0)
       (STEP1: Local.read_step th0 mem0 loc1 ts1 val1 released1 ord1 th1)
       (STEP2: Local.read_step th1 mem0 loc2 ts2 val2 released2 ord2 th2):
-  exists th1' th2',
+  exists th1',
     <<STEP1: Local.read_step th0 mem0 loc2 ts2 val2 released2 ord2 th1'>> /\
-    <<STEP2: Local.read_step th1' mem0 loc1 ts1 val1 released1 ord1 th2'>> /\
-    <<SIM: sim_local th2' th2>>.
+    <<STEP2: Local.read_step th1' mem0 loc1 ts1 val1 released1 ord1 th2>>.
 Proof.
-  inv STEP1. inv STEP2.
+  inv STEP1. inv STEP2. ss.
   exploit CommitFacts.read_min_spec; try apply WF0; try apply GET0; eauto.
   { eapply Snapshot.readable_mon; try apply COMMIT0; eauto. apply COMMIT. }
   i. des.
@@ -58,11 +48,10 @@ Proof.
   { eapply Snapshot.le_on_readable; eauto. apply COMMIT. }
   { apply WF0. }
   i. des.
-  eexists _, _. splits.
+  eexists. splits.
   - econs; eauto.
-  - econs; eauto.
-  - s. econs; s; try apply MemInv.sem_bot.
-    inv COMMIT. inv COMMIT0. inv MONOTONE. inv MONOTONE0.
+  - destruct th0. s. econs; try eapply CommitFacts.read_mon2; eauto.
+    s. inv COMMIT. inv COMMIT0. inv MONOTONE. inv MONOTONE0.
     unfold CommitFacts.read_min.
     destruct (Ordering.le Ordering.acquire ord2) eqn:ORD2'.
     { destruct ord2; ss. }
@@ -81,34 +70,33 @@ Qed.
 
 Lemma reorder_read_promise
       loc1 ts1 val1 released1 ord1
+      loc2 from2 to2 val2 released2
       th0 mem0
       th1
       th2 mem2
       (WF0: Local.wf th0 mem0)
       (STEP1: Local.read_step th0 mem0 loc1 ts1 val1 released1 ord1 th1)
-      (STEP2: Local.promise_step th1 mem0 th2 mem2):
-  exists th1' th2',
-    <<STEP1: Local.promise_step th0 mem0 th1' mem2>> /\
-    <<STEP2: Local.read_step th1' mem2 loc1 ts1 val1 released1 ord1 th2'>> /\
-    <<LOCAL: sim_local th2' th2>>.
+      (STEP2: Local.promise_step th1 mem0 loc2 from2 to2 val2 released2 th2 mem2):
+  exists th1',
+    <<STEP1: Local.promise_step th0 mem0 loc2 from2 to2 val2 released2 th1' mem2>> /\
+    <<STEP2: Local.read_step th1' mem2 loc1 ts1 val1 released1 ord1 th2>>.
 Proof.
   inv STEP1. inv STEP2. ss.
   exploit Memory.promise_future; try apply WF0; eauto. i. des.
   exploit Commit.future_wf; try apply WF0; eauto. i.
   exploit Memory.future_get; eauto. i.
   exploit CommitFacts.read_min_spec; try apply COMMIT; eauto. i. des.
-  eexists _, _. splits.
+  eexists. splits.
   - econs; try reflexivity; try apply MEMORY; eauto.
-  - econs; eauto. s.
-    match goal with
-    | [|- ?x = None] => destruct x eqn:X; auto
-    end.
-    eapply Memory.promise_get_inv in X; try apply MEMORY; try apply WF0; eauto.
-    des; [congruence|]. subst.
-    exploit Memory.promise_get1; try apply MEMORY; try apply WF0; eauto. i.
-    congruence.
-  - s. econs; s; try apply MemInv.sem_bot.
-    rewrite <- COMMIT0. apply CommitFacts.read_min_min. auto.
+  - destruct th0. ss. econs; try eapply CommitFacts.read_mon2; eauto.
+    + rewrite <- COMMIT0. apply CommitFacts.read_min_min. auto.
+    + match goal with
+      | [|- ?x = None] => destruct x eqn:X; auto
+      end.
+      eapply Memory.promise_get_inv in X; try apply MEMORY; try apply WF0; eauto.
+      des; [congruence|]. subst.
+      exploit Memory.promise_get1; try apply MEMORY; try apply WF0; eauto. i.
+      congruence.
 Qed.
 
 Lemma reorder_read_fulfill
@@ -122,11 +110,39 @@ Lemma reorder_read_fulfill
       (WF0: Local.wf th0 mem0)
       (STEP1: Local.read_step th0 mem0 loc1 ts1 val1 released1 ord1 th1)
       (STEP2: Local.fulfill_step th1 mem0 loc2 from2 to2 val2 released2 ord2 th2):
-  exists th1' th2',
+  exists th1',
     <<STEP1: Local.fulfill_step th0 mem0 loc2 from2 to2 val2 released2 ord2 th1'>> /\
-    <<STEP2: Local.read_step th1' mem0 loc1 ts1 val1 released1 ord1 th2'>> /\
-    <<SIM: sim_local th2' th2>>.
+    <<STEP2: Local.read_step th1' mem0 loc1 ts1 val1 released1 ord1 th2>>.
 Proof.
+  inv STEP1. inv STEP2. ss.
+  exploit Memory.fulfill_get; eauto. i.
+  exploit Memory.le_get; try apply WF0; eauto. i.
+  exploit CommitFacts.write_min_spec; try apply x1; try apply WF0; eauto.
+  { eapply Snapshot.writable_mon; try apply COMMIT0; eauto. apply COMMIT. }
+  { etransitivity; [apply COMMIT|]. apply COMMIT0. }
+  { instantiate (1 := ord2). i. inv COMMIT0.
+    rewrite <- RELEASED0; auto. apply Snapshot.incr_writes_mon. apply COMMIT.
+  }
+  { inv WF0. inv MEMORY0. exploit WF; eauto. }
+  i. des.
+  exploit CommitFacts.read_min_spec; try apply GET; eauto.
+  { eapply Snapshot.le_on_readable; eauto. apply COMMIT. }
+  { apply WF0. }
+  i. des.
+  eexists. splits.
+  - econs; eauto.
+  - destruct th0. ss. econs; try eapply CommitFacts.read_mon2; eauto.
+    + inv COMMIT. inv COMMIT0. inv MONOTONE. inv MONOTONE0. ss.
+      econs; committac.
+      * i. rewrite ACQUIRE; auto.
+      * rewrite CURRENT1. auto.
+      * rewrite READ0. apply CURRENT2.
+      * unfold LocFun.add, LocFun.find.
+        destruct (Loc.eq_dec loc loc2); committac.
+        etransitivity; [apply RELEASED|apply RELEASED4].
+      * rewrite ACQUIRABLE. auto.
+      * rewrite ACQUIRABLE0. auto.
+    + admit. (* promise get None *)
 Admitted.
 
 Lemma reorder_read_write
@@ -140,12 +156,21 @@ Lemma reorder_read_write
       (WF0: Local.wf th0 mem0)
       (STEP1: Local.read_step th0 mem0 loc1 ts1 val1 released1 ord1 th1)
       (STEP2: Local.write_step th1 mem0 loc2 from2 to2 val2 released2 ord2 th2 mem1):
-  exists th1' th2',
+  exists th1',
     <<STEP1: Local.write_step th0 mem0 loc2 from2 to2 val2 released2 ord2 th1' mem1>> /\
-    <<STEP2: Local.read_step th1' mem1 loc1 ts1 val1 released1 ord1 th2'>> /\
-    <<SIM: sim_local th2' th2>>.
+    <<STEP2: Local.read_step th1' mem1 loc1 ts1 val1 released1 ord1 th2>>.
 Proof.
-Admitted.
+  inv STEP2.
+  - exploit reorder_read_fulfill; eauto. i. des.
+    eexists. splits; eauto. econs 1. eauto.
+    inv STEP1. ss.
+  - exploit reorder_read_promise; eauto. i. des.
+    exploit reorder_read_fulfill; try apply FULFILL; eauto.
+    { eapply Local.promise_step_future; eauto. }
+    i. des.
+    eexists. splits; eauto. econs 2; eauto.
+    inv STEP1. ss.
+Qed.
 
 Lemma reorder_read_fence
       loc1 ts1 val1 released1 ord1
@@ -157,12 +182,41 @@ Lemma reorder_read_fence
       (WF0: Local.wf th0 mem0)
       (STEP1: Local.read_step th0 mem0 loc1 ts1 val1 released1 ord1 th1)
       (STEP2: Local.fence_step th1 mem0 ord2 th2):
-  exists th1' th2',
+  exists th1',
     <<STEP1: Local.fence_step th0 mem0 ord2 th1'>> /\
-    <<STEP2: Local.read_step th1' mem0 loc1 ts1 val1 released1 ord1 th2'>> /\
-    <<SIM: sim_local th2' th2>>.
+    <<STEP2: Local.read_step th1' mem0 loc1 ts1 val1 released1 ord1 th2>>.
 Proof.
-Admitted.
+  inv STEP1. inv STEP2. ss.
+  destruct (Ordering.le Ordering.acquire ord2) eqn:ORD2'.
+  { destruct ord2; ss. }
+  exploit CommitFacts.fence_min_spec; try apply WF0; eauto. i. des.
+  exploit CommitFacts.read_min_spec; try apply WF; try apply GET; eauto.
+  { instantiate (1 := ord2).
+    unfold CommitFacts.fence_min. rewrite ORD2'. ss. apply COMMIT.
+  }
+  { apply WF0. }
+  i. des.
+  eexists. splits.
+  - econs; eauto.
+  - destruct th0. s. econs; try eapply CommitFacts.read_mon2; eauto.
+    inv COMMIT. inv COMMIT0. inv MONOTONE. inv MONOTONE0.
+    unfold CommitFacts.read_min, CommitFacts.fence_min.
+    rewrite ORD2'. econs.
+    + destruct (Ordering.le Ordering.acquire ord1) eqn:ORD1; committac.
+      * rewrite ACQUIRE; auto.
+      * rewrite CURRENT0. auto.
+      * rewrite READ0. apply CURRENT1.
+      * rewrite CURRENT0. auto.
+      * rewrite READ0. apply CURRENT1.
+    + ss. i. unfold LocFun.find.
+      CommitFacts.condtac; committac.
+      * rewrite CURRENT0. eauto.
+      * etransitivity; [apply RELEASED|apply RELEASED0].
+      * etransitivity; [apply RELEASED|apply RELEASED0].
+    + ss. committac.
+      * rewrite ACQUIRABLE. auto.
+      * rewrite ACQUIRABLE0. auto.
+Qed.
 
 Lemma reorder_fulfill_read
       loc1 from1 to1 val1 released1 ord1
@@ -176,25 +230,60 @@ Lemma reorder_fulfill_read
       (WF0: Local.wf th0 mem0)
       (STEP1: Local.fulfill_step th0 mem0 loc1 from1 to1 val1 released1 ord1 th1)
       (STEP2: Local.read_step th1 mem0 loc2 ts2 val2 released2 ord2 th2):
-  exists th1' th2',
+  exists th1',
     <<STEP1: Local.read_step th0 mem0 loc2 ts2 val2 released2 ord2 th1'>> /\
-    <<STEP2: Local.fulfill_step th1' mem0 loc1 from1 to1 val1 released1 ord1 th2'>> /\
-    <<SIM: sim_local th2' th2>>.
+    <<STEP2: Local.fulfill_step th1' mem0 loc1 from1 to1 val1 released1 ord1 th2>>.
 Proof.
+  inv STEP1. inv STEP2. ss.
+  exploit Memory.fulfill_get; eauto. i.
+  exploit Memory.le_get; try apply WF0; eauto. i.
+  exploit CommitFacts.read_min_spec; try apply WF0; try apply GET; eauto.
+  { eapply Snapshot.readable_mon; try apply COMMIT0; eauto. apply COMMIT. }
+  i. des.
+  exploit CommitFacts.write_min_spec; try apply x1; eauto.
+  { eapply Snapshot.le_on_writable; eauto. apply COMMIT. }
+  { s. apply COMMIT. }
+  { instantiate (1 := ord1). destruct ord1; ss. }
+  { apply WF0. }
+  { inv WF0. inv MEMORY0. exploit WF0; eauto. }
+  i. des.
+  eexists. splits.
+  - econs; eauto.
+    admit. (* promise get None *)
+  - destruct th0. s. econs; try eapply CommitFacts.write_mon2; eauto.
+    inv COMMIT. inv COMMIT0. inv MONOTONE. inv MONOTONE0.
+    unfold CommitFacts.write_min, CommitFacts.read_min.
+    destruct (Ordering.le Ordering.acquire ord2) eqn:ORD2'; ss.
+    + econs; committac; auto.
+      * rewrite CURRENT1. auto.
+      * rewrite WRITE0. apply CURRENT2.
+      * unfold LocFun.add, LocFun.find.
+        CommitFacts.condtac; committac.
+        { rewrite RELEASED3. apply RELEASED4. }
+        { etransitivity; [apply RELEASED|apply RELEASED4]. }
+      * rewrite ACQUIRABLE0. auto.
+    + econs; committac; auto.
+      * rewrite CURRENT1. auto.
+      * rewrite WRITE0. apply CURRENT2.
+      * unfold LocFun.add, LocFun.find.
+        CommitFacts.condtac; committac.
+        { rewrite RELEASED3. apply RELEASED4. }
+        { etransitivity; [apply RELEASED|apply RELEASED4]. }
+      * rewrite ACQUIRABLE0. auto.
 Admitted.
 
 Lemma reorder_fulfill_promise
       loc1 from1 to1 val1 released1 ord1
+      loc2 from2 to2 val2 released2
       th0 mem0
       th1
       th2 mem2
       (WF0: Local.wf th0 mem0)
       (STEP1: Local.fulfill_step th0 mem0 loc1 from1 to1 val1 released1 ord1 th1)
-      (STEP2: Local.promise_step th1 mem0 th2 mem2):
-  exists th1' th2',
-    <<STEP1: Local.promise_step th0 mem0 th1' mem2>> /\
-    <<STEP2: Local.fulfill_step th1' mem2 loc1 from1 to1 val1 released1 ord1 th2'>> /\
-    <<LOCAL: sim_local th2' th2>>.
+      (STEP2: Local.promise_step th1 mem0 loc2 from2 to2 val2 released2 th2 mem2):
+  exists th1',
+    <<STEP1: Local.promise_step th0 mem0 loc2 from2 to2 val2 released2 th1' mem2>> /\
+    <<STEP2: Local.fulfill_step th1' mem2 loc1 from1 to1 val1 released1 ord1 th2>>.
 Proof.
 Admitted.
 
@@ -209,10 +298,9 @@ Lemma reorder_fulfill_fulfill
       (WF0: Local.wf th0 mem0)
       (STEP1: Local.fulfill_step th0 mem0 loc1 from1 to1 val1 released1 ord1 th1)
       (STEP2: Local.fulfill_step th1 mem0 loc2 from2 to2 val2 released2 ord2 th2):
-  exists th1' th2',
+  exists th1',
     <<STEP1: Local.fulfill_step th0 mem0 loc2 from2 to2 val2 released2 ord2 th1'>> /\
-    <<STEP2: Local.fulfill_step th1' mem0 loc1 from1 to1 val1 released1 ord1 th2'>> /\
-    <<SIM: sim_local th2' th2>>.
+    <<STEP2: Local.fulfill_step th1' mem0 loc1 from1 to1 val1 released1 ord1 th2>>.
 Proof.
 Admitted.
 
@@ -227,28 +315,46 @@ Lemma reorder_fulfill_write
       (WF0: Local.wf th0 mem0)
       (STEP1: Local.fulfill_step th0 mem0 loc1 from1 to1 val1 released1 ord1 th1)
       (STEP2: Local.write_step th1 mem0 loc2 from2 to2 val2 released2 ord2 th2 mem2):
-  exists th1' th2',
+  exists th1',
     <<STEP1: Local.write_step th0 mem0 loc2 from2 to2 val2 released2 ord2 th1' mem2>> /\
-    <<STEP2: Local.fulfill_step th1' mem2 loc1 from1 to1 val1 released1 ord1 th2'>> /\
-    <<SIM: sim_local th2' th2>>.
+    <<STEP2: Local.fulfill_step th1' mem2 loc1 from1 to1 val1 released1 ord1 th2>>.
 Proof.
+  inv STEP2.
+  - exploit reorder_fulfill_fulfill; eauto. i. des.
+    eexists. splits; eauto. econs 1. eauto.
+    admit. (* promise None *)
+  - exploit reorder_fulfill_promise; eauto. i. des.
+    exploit reorder_fulfill_fulfill; try apply STEP2; eauto.
+    { eapply Local.promise_step_future; eauto. }
+    i. des.
+    eexists. splits; eauto. econs 2; eauto.
+    admit. (* promise None *)
 Admitted.
 
 Lemma reorder_fence_promise
       ord1
+      loc2 from2 to2 val2 released2
       th0 mem0
       th1
       th2 mem2
       (ORD1: Ordering.le ord1 Ordering.acquire)
       (WF0: Local.wf th0 mem0)
       (STEP1: Local.fence_step th0 mem0 ord1 th1)
-      (STEP2: Local.promise_step th1 mem0 th2 mem2):
-  exists th1' th2',
-    <<STEP1: Local.promise_step th0 mem0 th1' mem2>> /\
-    <<STEP2: Local.fence_step th1' mem2 ord1 th2'>> /\
-    <<SIM: sim_local th2' th2>>.
+      (STEP2: Local.promise_step th1 mem0 loc2 from2 to2 val2 released2 th2 mem2):
+  exists th1',
+    <<STEP1: Local.promise_step th0 mem0 loc2 from2 to2 val2 released2 th1' mem2>> /\
+    <<STEP2: Local.fence_step th1' mem2 ord1 th2>>.
 Proof.
-Admitted.
+  inv STEP1. inv STEP2. ss.
+  exploit Memory.promise_future; try apply WF0; eauto. i. des.
+  exploit Commit.future_wf; try apply WF0; eauto. i.
+  exploit CommitFacts.fence_min_spec; try apply COMMIT; eauto. i. des.
+  eexists. splits.
+  - econs; try reflexivity; try apply MEMORY; eauto.
+  - destruct th0. ss. econs; try eapply CommitFacts.fence_mon2; eauto.
+    + rewrite <- COMMIT0. apply CommitFacts.fence_min_min. auto.
+    + s. econs. destruct ord1; ss.
+Qed.
 
 Lemma reorder_fence_fulfill
       ord1
@@ -260,12 +366,39 @@ Lemma reorder_fence_fulfill
       (WF0: Local.wf th0 mem0)
       (STEP1: Local.fence_step th0 mem0 ord1 th1)
       (STEP2: Local.fulfill_step th1 mem0 loc2 from2 to2 val2 released2 ord2 th2):
-  exists th1' th2',
+  exists th1',
     <<STEP1: Local.fulfill_step th0 mem0 loc2 from2 to2 val2 released2 ord2 th1'>> /\
-    <<STEP2: Local.fence_step th1' mem0 ord1 th2'>> /\
-    <<SIM: sim_local th2' th2>>.
+    <<STEP2: Local.fence_step th1' mem0 ord1 th2>>.
 Proof.
-Admitted.
+  destruct (Ordering.le Ordering.release ord1) eqn:ORD1'.
+  { destruct ord1; ss. }
+  inv STEP1. inv STEP2. ss.
+  exploit Memory.fulfill_get; eauto. i.
+  exploit Memory.le_get; try apply WF0; eauto. i.
+  exploit CommitFacts.write_min_spec; try apply x1; try apply WF0; eauto.
+  { eapply Snapshot.writable_mon; try apply COMMIT0; eauto. apply COMMIT. }
+  { etransitivity; [apply COMMIT|]. apply COMMIT0. }
+  { instantiate (1 := ord2). i. inv COMMIT0.
+    rewrite <- RELEASED0; auto. apply Snapshot.incr_writes_mon. apply COMMIT.
+  }
+  { inv WF0. inv MEMORY1. exploit WF; eauto. }
+  i. des.
+  exploit CommitFacts.fence_min_spec; eauto.
+  { apply WF0. }
+  i. des.
+  eexists. splits.
+  - econs; eauto.
+  - destruct th0. ss. econs; try eapply CommitFacts.fence_mon2; eauto.
+    + inv COMMIT. inv COMMIT0. inv MONOTONE. inv MONOTONE0. ss.
+      econs; committac.
+      * rewrite ACQUIRE; auto.
+      * rewrite CURRENT0. auto.
+      * unfold LocFun.add, LocFun.find. rewrite ORD1'.
+        CommitFacts.condtac; committac.
+        etransitivity; [apply RELEASED|apply RELEASED4].
+      * rewrite ACQUIRABLE. auto.
+    + s. econs. destruct ord1; ss.
+Qed.
 
 Lemma reorder_fence_write
       ord1
@@ -277,244 +410,18 @@ Lemma reorder_fence_write
       (WF0: Local.wf th0 mem0)
       (STEP1: Local.fence_step th0 mem0 ord1 th1)
       (STEP2: Local.write_step th1 mem0 loc2 from2 to2 val2 released2 ord2 th2 mem2):
-  exists th1' th2',
+  exists th1',
     <<STEP1: Local.write_step th0 mem0 loc2 from2 to2 val2 released2 ord2 th1' mem2>> /\
-    <<STEP2: Local.fence_step th1' mem2 ord1 th2'>> /\
-    <<SIM: sim_local th2' th2>>.
+    <<STEP2: Local.fence_step th1' mem2 ord1 th2>>.
 Proof.
+  inv STEP2.
+  - exploit reorder_fence_fulfill; eauto. i. des.
+    eexists. splits; eauto. econs 1. eauto.
+    admit. (* promise None *)
+  - exploit reorder_fence_promise; eauto. i. des.
+    exploit reorder_fence_fulfill; try apply STEP2; eauto.
+    { eapply Local.promise_step_future; eauto. }
+    i. des.
+    eexists. splits; eauto. econs 2; eauto.
+    admit. (* promise None *)
 Admitted.
-
-
-
-
-(* Lemma sim_fulfill_promise *)
-(*       loc from to val released ord *)
-(*       th1_src mem1_src *)
-(*       th1_tgt mem1_tgt *)
-(*       th2_tgt mem2_tgt *)
-(*       (ORD: Ordering.le ord Ordering.relaxed) *)
-(*       (LOCAL1: sim_fulfill loc from to val released ord th1_src th1_tgt) *)
-(*       (MEMORY1: sim_memory mem1_src mem1_tgt) *)
-(*       (WF1_SRC: Local.wf th1_src mem1_src) *)
-(*       (WF1_TGT: Local.wf th1_tgt mem1_tgt) *)
-(*       (STEP_TGT: Local.promise_step th1_tgt mem1_tgt th2_tgt mem2_tgt): *)
-(*   exists th2_src mem2_src, *)
-(*     <<STEP_SRC: Local.promise_step th1_src mem1_src th2_src mem2_src>> /\ *)
-(*     <<LOCAL2: sim_fulfill loc from to val released ord th2_src th2_tgt>> /\ *)
-(*     <<MEMORY2: sim_memory mem2_src mem2_tgt>>. *)
-(* Proof. *)
-(*   inv LOCAL1. inv STEP_TGT. *)
-(*   exploit MemInv.promise; eauto. *)
-(*   { apply WF1_SRC. } *)
-(*   { apply WF1_TGT. } *)
-(*   i. des. *)
-(*   exploit Memory.promise_future; try apply PROMISE_SRC; eauto. *)
-(*   { apply WF1_SRC. } *)
-(*   { apply WF1_SRC. } *)
-(*   i. des. *)
-(*   eexists _, _. splits; eauto. *)
-(*   - econs; eauto. *)
-(*     + reflexivity. *)
-(*     + eapply Commit.future_wf; eauto. apply WF1_SRC. *)
-(*   - econs; s; eauto. etransitivity; eauto. *)
-(* Qed. *)
-
-(* Lemma sim_fulfill_read *)
-(*       loc1 from1 to1 val1 released1 ord1 *)
-(*       loc2 ts2 val2 released2 ord2 *)
-(*       th1_src mem1_src *)
-(*       th1_tgt mem1_tgt *)
-(*       th2_tgt *)
-(*       (LOC: loc1 <> loc2) *)
-(*       (ORD1: Ordering.le ord1 Ordering.relaxed) *)
-(*       (ORD2: Ordering.le ord2 Ordering.release) *)
-(*       (LOCAL1: sim_fulfill loc1 from1 to1 val1 released1 ord1 th1_src th1_tgt) *)
-(*       (MEMORY1: sim_memory mem1_src mem1_tgt) *)
-(*       (WF1_SRC: Local.wf th1_src mem1_src) *)
-(*       (WF1_TGT: Local.wf th1_tgt mem1_tgt) *)
-(*       (STEP_TGT: Local.read_step th1_tgt mem1_tgt loc2 ts2 val2 released2 ord2 th2_tgt): *)
-(*   exists th2_src, *)
-(*     <<STEP_SRC: Local.read_step th1_src mem1_src loc2 ts2 val2 released2 ord2 th2_src>> /\ *)
-(*     <<LOCAL2: sim_fulfill loc1 from1 to1 val1 released1 ord1 th2_src th2_tgt>>. *)
-(* Proof. *)
-(*   inv LOCAL1. inv STEP_TGT. *)
-(*   exploit Memory.le_get. *)
-(*   { apply WF1_SRC. } *)
-(*   { inv PROMISE. eapply Memory.le_get. *)
-(*     - apply Memory.le_join_r. memtac. *)
-(*     - apply Memory.singleton_get. *)
-(*   } *)
-(*   intro GET1_SRC. *)
-(*   exploit Memory.splits_get; try apply GET; eauto. *)
-(*   { apply MEMORY1. } *)
-(*   intro GET2_SRC. *)
-(*   exploit CommitFacts.read_min_spec; try apply GET2_SRC; eauto. *)
-(*   { inv COMMIT. eapply Snapshot.readable_mon; eauto. *)
-(*     etransitivity; [|apply COMMIT2]. apply COMMIT1. *)
-(*   } *)
-(*   { apply WF1_SRC. } *)
-(*   { apply WF1_SRC. } *)
-(*   i. des. *)
-(*   destruct (Ordering.le Ordering.release ord1) eqn:ORD1'. *)
-(*   { destruct ord1; ss. } *)
-(*   assert (RELEASED_SRC: Memory.wf_snapshot released1 mem1_src). *)
-(*   { inv WF1_SRC. inv MEMORY. exploit WF0; try apply GET1_SRC; eauto. } *)
-(*   exploit CommitFacts.write_min_spec; try apply RELEASED_SRC; eauto. *)
-(*   { eapply Snapshot.le_on_writable; eauto. apply COMMIT1. } *)
-(*   { ss. inv COMMIT1. etransitivity; eauto. apply MONOTONE. } *)
-(*   { instantiate (1 := ord1). destruct ord1; ss. } *)
-(*   { apply WF1_SRC. } *)
-(*   i. des. *)
-(*   eexists _. splits; eauto. *)
-(*   - econs; eauto. inv PROMISE. *)
-(*     match goal with *)
-(*     | [|- ?x = None] => destruct x eqn:X; auto *)
-(*     end. *)
-(*     apply Memory.join_get in X; memtac; try congruence. *)
-(*     apply Memory.singleton_get_inv in X. des. congruence. *)
-(*   - econs; eauto. s. *)
-(*     exploit CommitFacts.write_min_min; try apply COMMIT1; eauto. i. *)
-(*     exploit CommitFacts.read_min_min; try apply COMMIT; eauto. i. *)
-(*     unfold CommitFacts.read_min in *. *)
-(*     destruct (Ordering.le Ordering.acquire ord2) eqn:ORD2'. *)
-(*     { destruct ord2; ss. } *)
-(*     inv x0. inv x1. *)
-(*     apply Snapshot.incr_writes_inv in CURRENT1. *)
-(*     apply Snapshot.incr_reads_inv in CURRENT2. des. *)
-(*     econs; ss. *)
-(*     + apply Snapshot.incr_writes_spec. *)
-(*       * apply Snapshot.incr_reads_spec; ss. *)
-(*         etransitivity; [apply COMMIT1|]. *)
-(*         etransitivity; [apply COMMIT2|]. *)
-(*         apply COMMIT. *)
-(*       * etransitivity; [apply COMMIT1|]. *)
-(*         etransitivity; [apply COMMIT2|]. *)
-(*         apply COMMIT. *)
-(*     + i. unfold LocFun.add, LocFun.find. *)
-(*       destruct (Loc.eq_dec loc loc1). *)
-(*       * subst. rewrite ORD1'. *)
-(*         etransitivity; [apply COMMIT1|]. *)
-(*         etransitivity; [apply COMMIT2|]. *)
-(*         apply COMMIT. *)
-(*       * etransitivity; [apply COMMIT1|]. *)
-(*         etransitivity; [apply COMMIT2|]. *)
-(*         apply COMMIT. *)
-(*     + etransitivity; eauto. *)
-(*       apply Snapshot.join_spec. *)
-(*       * apply Snapshot.join_l. *)
-(*       * etransitivity; [|apply Snapshot.join_r]. *)
-(*         etransitivity; [apply COMMIT1|]. *)
-(*         apply COMMIT2. *)
-(* Qed. *)
-
-(* Lemma sim_fulfill_write *)
-(*       loc1 from1 to1 val1 released1 ord1 *)
-(*       loc2 from2 to2 val2 released2 ord2 *)
-(*       th1_src mem1_src *)
-(*       th1_tgt mem1_tgt *)
-(*       th2_tgt mem2_tgt *)
-(*       (LOC: loc1 <> loc2) *)
-(*       (ORD1: Ordering.le ord1 Ordering.relaxed) *)
-(*       (LOCAL1: sim_fulfill loc1 from1 to1 val1 released1 ord1 th1_src th1_tgt) *)
-(*       (MEMORY1: sim_memory mem1_src mem1_tgt) *)
-(*       (WF1_SRC: Local.wf th1_src mem1_src) *)
-(*       (WF1_TGT: Local.wf th1_tgt mem1_tgt) *)
-(*       (STEP_TGT: Local.write_step th1_tgt mem1_tgt loc2 from2 to2 val2 released2 ord2 th2_tgt mem2_tgt): *)
-(*   exists th2_src mem2_src, *)
-(*     <<STEP_SRC: Local.write_step th1_src mem1_src loc2 from2 to2 val2 released2 ord2 th2_src mem2_src>> /\ *)
-(*     <<LOCAL2: sim_fulfill loc1 from1 to1 val1 released1 ord1 th2_src th2_tgt>> /\ *)
-(*     <<MEMORY2: sim_memory mem2_src mem2_tgt>>. *)
-(* Proof. *)
-(*   destruct (Ordering.le Ordering.release ord1) eqn:ORD1'. *)
-(*   { destruct ord1; ss. } *)
-(*   inv LOCAL1. inv STEP_TGT. *)
-(*   exploit MemInv.write; eauto. *)
-(*   { apply WF1_SRC. } *)
-(*   { apply WF1_TGT. } *)
-(*   { inv PROMISE. unfold Memory.join. *)
-(*     unfold Memory.singleton, LocFun.add, LocFun.find. *)
-(*     destruct (Loc.eq_dec loc2 loc1); [congruence|]. *)
-(*     unfold LocFun.init. rewrite Cell.bot_join. auto. *)
-(*   } *)
-(*   i. des. *)
-(*   exploit Memory.write_future; try apply WRITE_SRC; eauto. *)
-(*   { apply WF1_SRC. } *)
-(*   { apply WF1_SRC. } *)
-(*   i. des. *)
-(*   exploit Memory.write_get; try apply WRITE_SRC; eauto. *)
-(*   { apply WF1_SRC. } *)
-(*   intro GET2_SRC. *)
-(*   exploit CommitFacts.write_min_spec; eauto. *)
-(*   { eapply Snapshot.writable_mon; [|apply COMMIT]. *)
-(*     etransitivity; [|apply COMMIT2]. apply COMMIT1. *)
-(*   } *)
-(*   { etransitivity; [apply COMMIT1|]. *)
-(*     etransitivity; [apply COMMIT2|]. *)
-(*     etransitivity; [apply COMMIT|]. apply COMMIT. *)
-(*   } *)
-(*   { instantiate (1 := ord2). inv COMMIT. i. *)
-(*     rewrite <- RELEASED, <- RELEASE; auto. *)
-(*     apply Snapshot.incr_writes_spec; auto. *)
-(*     etransitivity; [apply COMMIT1|]. *)
-(*     etransitivity; [apply COMMIT2|]. *)
-(*     apply MONOTONE. *)
-(*   } *)
-(*   { eapply Commit.future_wf; eauto. apply WF1_SRC. } *)
-(*   { inv WF2. exploit WF; eauto. } *)
-(*   i. des. *)
-(*   exploit Memory.le_get. *)
-(*   { apply WF1_SRC. } *)
-(*   { inv PROMISE. eapply Memory.le_get. *)
-(*     - apply Memory.le_join_r. memtac. *)
-(*     - apply Memory.singleton_get. *)
-(*   } *)
-(*   intro GET1_SRC. *)
-(*   exploit Memory.future_get; try apply GET1_SRC; eauto. *)
-(*   intro GET1_SRC'. *)
-(*   exploit CommitFacts.write_min_spec; try apply GET1_SRC'; eauto. *)
-(*   { eapply Snapshot.le_on_writable; eauto. apply COMMIT1. } *)
-(*   { inv COMMIT1. rewrite <- RELEASED, RELEASED1; auto. *)
-(*     apply MONOTONE. *)
-(*   } *)
-(*   { instantiate (1 := ord1). destruct ord1; ss. } *)
-(*   { inv WF2. exploit WF0; eauto. } *)
-(*   i. des. *)
-(*   eexists _, _. splits; eauto. *)
-(*   - econs; eauto. *)
-(*   - econs; eauto. s. *)
-(*     exploit CommitFacts.write_min_min; try apply COMMIT1; eauto. i. *)
-(*     exploit CommitFacts.write_min_min; try apply COMMIT; eauto. i. *)
-(*     inv x0. inv x1. *)
-(*     apply Snapshot.incr_writes_inv in CURRENT1. *)
-(*     apply Snapshot.incr_writes_inv in CURRENT2. des. *)
-(*     econs; ss. *)
-(*     + repeat apply Snapshot.incr_writes_spec; ss. *)
-(*       * etransitivity; [apply COMMIT1|]. *)
-(*         etransitivity; [apply COMMIT2|]. *)
-(*         apply COMMIT. *)
-(*       * etransitivity; [apply COMMIT1|]. *)
-(*         etransitivity; [apply COMMIT2|]. *)
-(*         apply COMMIT. *)
-(*     + i. unfold LocFun.add, LocFun.find. rewrite ORD1'. *)
-(*       etransitivity; [|apply RELEASED2]. *)
-(*       unfold LocFun.add, LocFun.find. *)
-(*       destruct (Loc.eq_dec loc loc1). *)
-(*       * subst. destruct (Loc.eq_dec loc1 loc2); [congruence|]. *)
-(*         etransitivity; [apply COMMIT1|]. apply COMMIT2. *)
-(*       * destruct (Loc.eq_dec loc loc2). *)
-(*         { subst. *)
-(*           match goal with *)
-(*           | [|- context[if ?c then _ else _]] => destruct c *)
-(*           end. *)
-(*           - apply Snapshot.join_spec. *)
-(*             + etransitivity; [|apply Snapshot.join_l]. *)
-(*               apply Snapshot.incr_writes_mon. *)
-(*               etransitivity; [apply COMMIT1|]. apply COMMIT2. *)
-(*             + etransitivity; [|apply Snapshot.join_r]. *)
-(*               etransitivity; [apply COMMIT1|]. apply COMMIT2. *)
-(*           - etransitivity; [apply COMMIT1|]. apply COMMIT2. *)
-(*         } *)
-(*         { etransitivity; [apply COMMIT1|]. apply COMMIT2. } *)
-(*     + etransitivity; [apply COMMIT1|]. *)
-(*       etransitivity; [apply COMMIT2|]. eauto. *)
-(* Qed. *)
